

DFOCC: DF-CCSD(T) equations

Reference: DFOCC in Psi4 by Uğur Bozkaya (performs density-fitted orbital-optimized CC calculations)

1 Notations

Four-index integral (in chemists' notation):

$$(pq|rs) = \sum_Q B_{pq}^Q B_{rs}^Q, \quad (1)$$

Four-index integral (in physicists' notation):

$$\langle pr|qs \rangle = \sum_Q B_{pq}^Q B_{rs}^Q, \quad (2)$$

where B_{pq}^Q is the three-index density fitting integral.

Orbital and Basis Information:

- Number of doubly occupied orbitals (i, j, \dots) : N_O
- Number of virtual orbitals (a, b, \dots) : N_V
- Number of molecular orbitals: $N_O + N_V$
- Number of auxiliary basis functions (Q) : N_{aux}
- Orbital energy of orbital p : ϵ_p

2 3-index intermediates

First, we construct three-index intermediates that are used in \hat{T}_1 and \hat{T}_2 equations. The intermediates in Table 1. will be used in the following sections.

Table 1: Explicit expression of three-index intermediates.

$\mathbf{T}_{\mathbf{ia}}^{\mathbf{Q}} = \sum_{jb} B_{jb}^{\mathbf{Q}} u_{ij}^{ab}$, where $u_{ij}^{ab} = 2t_{ij}^{ab} - t_{ij}^{ba}$
$\mathbf{t}^{\mathbf{Q}} = 2 \sum_{mf} t_m^f B_{mf}^{\mathbf{Q}}$
$\mathbf{t}_{ij}^{\mathbf{Q}} = \sum_e t_i^e t_{je}^{\mathbf{Q}}$, $\mathbf{t}_{\mathbf{ia}}^{\mathbf{Q}} = \sum_e t_i^e t_{fa}^{\mathbf{Q}}$, $\mathbf{t}_{\mathbf{ai}}^{\mathbf{Q}} = \sum_e t_m^a t_{mi}^{\mathbf{Q}}$, $\mathbf{t}_{\mathbf{ab}}^{\mathbf{Q}} = \sum_e t_m^a t_{mb}^{\mathbf{Q}}$
$\tilde{\mathbf{T}}_{\mathbf{ia}}^{\mathbf{Q}} = \sum_m t_m^a t_{im}^{\mathbf{Q}}$
$\mathbf{t}'_{\mathbf{ia}}^{\mathbf{Q}} = t_{ia}^{\mathbf{Q}} - t_{ai}^{\mathbf{Q}} - \tilde{\mathbf{T}}_{\mathbf{ia}}^{\mathbf{Q}}$
$\mathbf{Tau}_{\mathbf{ia}}^{\mathbf{Q}} = \sum_{mf} (2\tau_{im}^{af} - \tau_{mi}^{af}) B_{mf}^{\mathbf{Q}}$, where $\tau_{ij}^{ab} = \frac{1}{2} t_i^a t_j^b$
$\mathbf{Tau}'_{\mathbf{ia}}^{\mathbf{Q}} = t_{ia}^{\mathbf{Q}} + \mathbf{Tau}_{\mathbf{ia}}^{\mathbf{Q}}$
$\mathbf{Tau}''_{\mathbf{ia}}^{\mathbf{Q}} = -t_{ia}^{\mathbf{Q}} + \mathbf{Tau}_{\mathbf{ia}}^{\mathbf{Q}}$

Table 2: t_1 -transformed Fock matrix blocks

$\mathbf{F}_{\mathbf{ov}} \Rightarrow \mathbf{F}_{\mathbf{me}} = \sum_Q B_{me}^{\mathbf{Q}} t^{\mathbf{Q}} - \sum_{Qn} t_{nm}^{\mathbf{Q}} B_{ne}^{\mathbf{Q}}$
$\mathbf{F}_{\mathbf{oo}} \Rightarrow \mathbf{F}_{\mathbf{mi}} = \sum_Q B_{mi}^{\mathbf{Q}} t^{\mathbf{Q}} + \sum_{Qe} \mathbf{Tau}''_{ie}^{\mathbf{Q}} B_{me}^{\mathbf{Q}} + \frac{1}{2} \sum_e t_i^e F_{me}$
$\mathbf{F}_{\mathbf{vv}} \Rightarrow \mathbf{F}_{\mathbf{ae}} = \sum_Q B_{me}^{\mathbf{Q}} t^{\mathbf{Q}} - \sum_{Qm} \mathbf{Tau}'_{ma}^{\mathbf{Q}} B_{me}^{\mathbf{Q}} - \frac{1}{2} \sum_m t_m^a F_{me}$

3 \hat{T}_1 equation

3.1 F intermediates

3.2 \hat{T}_1 residual

The terms are arranged to match Equation (19)-(22)

$$\begin{aligned}
R_i^a &= \sum_e F_{ae} t_i^e - \sum_m t_m^a F_{mi} \Rightarrow F_{ai} \\
&+ \sum_Q t^{\mathbf{Q}} B_{ia}^{\mathbf{Q}} + \sum_{Qe} T_{ie}^{\mathbf{Q}} B_{ea}^{\mathbf{Q}} \Rightarrow A_i^a \\
&- \sum_{Qm} (T_{ma}^{\mathbf{Q}} + t_{ma}^{\mathbf{Q}}) B_{mi}^{\mathbf{Q}} \Rightarrow B_i^a \\
&+ \sum_{me} u_{im}^{ae} F_{me} \Rightarrow C_i^a
\end{aligned} \tag{3}$$

Update the \hat{T}_1 amplitude,

$$t_i^a = t_i^a + R_i^a / D_i^a. \tag{4}$$

The denominator is defined as

$$D_i^a = \epsilon_a - \epsilon_i, \tag{5}$$

where ϵ_p is the orbital energy of the orbital p .

Note that t_1 -dressed $B_{pq}^{\mathbf{Q}}$ integrals are not explicitly computed as described in the reference, but arranged into the equations with t_1 and bare $B_{pq}^{\mathbf{Q}}$.

4 \hat{T}_2 equation

4.1 Four-index intermediates

Table 3: Two-particle excitation terms

$\mathbf{u}_{ij}^{ab} = 2t_{ij}^{ab} - t_{ji}^{ab}$
$\mathbf{Tau}_{ij}^{ab} = t_{ij}^{ab} + t_i^a t_j^b$
$\tilde{\mathbf{Tau}}_{ij}^{ab} = t_{ij}^{ab} + \frac{1}{2} t_i^a t_j^b$

4.2 $\mathbf{W}_{mnij} \mathbf{T}_2 \rightarrow \mathbf{R}_{ij}^{ab}$

$$W_{mnij} = \langle mn|ij \rangle + \sum_Q (t_{im}^Q B_{jn}^Q + t_{jn}^Q B_{im}^Q) + \sum_{ef} Tau_{ij}^{ef} \langle mn|ef \rangle \quad (6)$$

- For the first term, the two-electron integral (TEI) is calculated as

$$W_{mnij} = \langle mn|ij \rangle = \sum_Q B_{im}^Q B_{jn}^Q. \quad (7)$$

- For the second term, we have

$$X_{ij}^{mn} = \sum_Q t_{im}^Q B_{jn}^Q \quad (8)$$

and then

$$W_{mnij} + = P_{ij}^{mn} X_{ij}^{mn}, \quad (9)$$

where P_{ij}^{ab} is the permutation operator defined as $P_{ij}^{ab} X_{ij}^{ab} = X_{ij}^{ab} + X_{ji}^{ba}$.

- For the third term, the packed symmetric(+) and antisymmetric(-) four-index tensor is utilized for both Tau_{ij}^{ef} and $\langle mn|ef \rangle$ for an efficient algorithm. Define the symmetric and antisymmetric operators as

$$\hat{S} \equiv \frac{1}{2}(\hat{I} + \hat{P}) \quad (10)$$

and

$$\hat{A} \equiv \frac{1}{2}(\hat{I} - \hat{P}) \quad (11)$$

respectively, where \hat{I} is the identity operator and $\hat{P} X_{ij}^{ab} = X_{ji}^{ab}$ or X_{ij}^{ba} so that $\hat{P}^2 = \hat{I}$. To achieve more savings, the summation can be limited to $i \geq j$ and $a \geq b$ for a tensor X_{ij}^{ab} .

Tau_{ij}^{ef} :

$$(+)\tau_{i \geq j}^{a \geq b} = \frac{1}{2}(Tau_{ij}^{ef} + Tau_{ji}^{ef})(2 - \delta_{ef}) \quad (12)$$

$$(-)\tau_{i \geq j}^{a \geq b} = \frac{1}{2}(Tau_{ij}^{ef} - Tau_{ji}^{ef})(2 - \delta_{ef}) \quad (13)$$

$\langle mn|ef \rangle \Rightarrow V_{mn}^{ef}$:

$$V_{mn}^{e \geq f} = \sum_Q B_{me}^Q B_{nf}^Q \quad (14)$$

$$(+)\tau_{m \geq n}^{e \geq f} = \frac{1}{2}(V_{mn}^{ef} + V_{nm}^{ef}) \quad (15)$$

$$(-)V_{m \geq n}^{e \geq f} = \frac{1}{2}(V_{mn}^{ef} - V_{nm}^{ef}) \quad (16)$$

W_{mnij} :

$$(+)W_{mnij} (m \geq n, i \geq j) = \sum_{e \geq f} (+)Tau_{i \geq j}^{e \geq f} (+)V_{m \geq n}^{e \geq f} \quad (17)$$

$$(-)W_{mnij} (m \geq n, i \geq j) = \sum_{e \geq f} (-)Tau_{i \geq j}^{e \geq f} (-)V_{m \geq n}^{e \geq f} \quad (18)$$

$$W_{mnij} + = (+)W_{mnij} + \epsilon_{mn}\epsilon_{ij}(-)W_{mnij}, \quad (19)$$

where

$$\epsilon_{pq} = \begin{cases} 1 & \text{if } p \geq q \\ -1 & \text{if } p < q \end{cases} \quad (20)$$

The same technique can be applied to the contraction between W_{mnij} and the \hat{T}_2 amplitude in the next step.

$$S(W_{mnij}) = \frac{1}{2}(W_{mnij} + W_{nmij}) \quad (21)$$

$$A(W_{mnij}) = \frac{1}{2}(W_{mnij} - W_{nmij}) \quad (22)$$

$$S_{i \geq j}^{a \geq b} = \sum_{m \geq n} (+)Tau_{m \geq n}^{a \geq b} S(W_{mnij})_{m \geq n, i \geq j} \quad (23)$$

$$A_{i \geq j}^{a \geq b} = \sum_{m \geq n} (-)Tau_{m \geq n}^{a \geq b} A(W_{mnij})_{m \geq n, i \geq j} \quad (24)$$

Finally, we have the contribution to the \hat{T}_2 residual as

$$\sum_{mn} Tau_{mn}^{ab} W_{mnij} \Rightarrow S_{ij}^{ab} + \epsilon_{ij}\epsilon_{ab}A_{ij}^{ab} \rightarrow R_{ij}^{ab}. \quad (25)$$

Note that limiting the summation to $e \geq f$ in Eq. 12 reduces the cost of the construction of the four-index tensor by a factor 2. The cost of the contraction with the CC amplitudes is reduced by a factor 4 as shown in Eq. 15, 16 and Eq. 21, 22.

4.3 $W_{mbej}T_2 \rightarrow R_{ij}^{ab}$

We first calculate

$$W_{mbej} = \langle mb|ej\rangle + \sum_Q (t'_{jb}^Q + \frac{1}{2}T_{jb}^Q)B_{me}^Q - \frac{1}{2}\sum_{nf} t_{jn}^{bf}\langle mn|ef\rangle, \quad (26)$$

where the TEIs are calculated as

$$\langle mb|ej\rangle = \sum_Q B_{me}^Q B_{jb}^Q \quad (27)$$

and

$$\langle mn|ef\rangle = \sum_Q B_{me}^Q B_{nf}^Q. \quad (28)$$

And then we calculate

$$W'_{mbej} = \langle me|jb\rangle + X_{jm}^{be} - \frac{1}{2}\sum_{nf} \langle mn|ef\rangle t_{nj}^{bf}, \quad (29)$$

where

$$\langle me|jb\rangle = \sum_Q B_{mj}^Q B_{eb}^Q, \quad (30)$$

$$\langle mn|ef\rangle = \sum_Q B_{me}^Q B_{nf}^Q, \quad (31)$$

and

$$X_{jm}^{be} = - \sum_Q t_{be}^Q (t_{jm}^Q + B_{jm}^Q) + \sum_Q t_{jm}^Q B_{be}^Q \quad (32)$$

With W_{mbej} and W'_{mbej} , we construct

$$C_{ij}^{ab} = - \sum_{me} t_{mi}^{ae} W'_{mbej}, \quad (33)$$

$$\tilde{C}_{ij}^{ab} = \frac{1}{2} (C_{ij}^{ab} + C_{ji}^{ba}), \quad (34)$$

and

$$D_{ij}^{ab} = \frac{1}{2} \sum_{me} u_{im}^{ae} (2W_{mbej} - W'_{mbej}). \quad (35)$$

The contribution to the \hat{T}_2 residual is obtained from

$$(\tilde{C}_{ij}^{ab} + 2\tilde{C}_{ij}^{ba}) + (D_{ij}^{ab} + D_{ji}^{ba}) \rightarrow R_{ij}^{ab}. \quad (36)$$

4.4 $\mathbf{W_{ijam}T_2 \rightarrow R_{ij}^{ab}}$

$$W_{ijam} = \sum_{ef} Tau_{ij}^{ef} \langle am|ef \rangle \quad (37)$$

Both Tau_{ij}^{ef} and $\langle am|ef \rangle$ are constructed using packed symmetric and antisymmetric four-index tensors as described in section 4.1. For $\langle am|ef \rangle$ specifically, since it contains three virtual indices, the three-index intermediate for a fixed m is calculated to avoid storing the whole set of $N_O N_V^3$ tensors. Its contribution to W_{mnij} for a fixed m is then calculated in each loop.

$\langle am|ef \rangle$ with fixed m is calculated as

$$V_{ae,f}^{[m]} = \sum_Q B_{ae}^Q B_{[m]f}^Q \quad (38)$$

The symmetric and antisymmetric tensors are constructed as

$$(+)V_{ae,f}^{[m]} = \frac{1}{2} (V_{ae,f}^{[m]} + V_{af,e}^{[m]}) \quad (39)$$

and

$$(-)V_{ae,f}^{[m]} = \frac{1}{2} (V_{ae,f}^{[m]} - V_{af,e}^{[m]}) \quad (40)$$

respectively. For the contraction with the \hat{T}_2 amplitude, we have

$$S_{i \geq j, a}^{[m]} = \sum_{e \geq f} (+) Tau_{i \geq j}^{e \geq f} (+) V_{a, e \geq f}^{[m]} \quad (41)$$

$$A_{i \geq j, a}^{[m]} = \sum_{e \geq f} (-) Tau_{i \geq j}^{e \geq f} (-) V_{a, e \geq f}^{[m]} \quad (42)$$

After looping over m , we obtain $S_{i \geq j, am}$ and $A_{i \geq j, am}$ as symmetric and antisymmetric tensors for W_{ijam} when $i \geq j$.

$$W_{ijam} = S_{i \geq j, am} + \epsilon_{ij} A_{i \geq j, am} \quad (43)$$

Its contribution to the residual is calculated as

$$X_{ij}^{ab} = - \sum_m t_m^b W_{ijam} \quad (44)$$

$$X_{ij}^{ab} + X_{ji}^{ba} \rightarrow R_{ij}^{ab} \quad (45)$$

4.5 $W_{abef}T_2 \rightarrow R_{ij}^{ab}$

In this part, the four-virtual-index tensor $\langle ab|ef \rangle$ is needed. To avoid constructing and storing the whole set of N_V^4 tensor, three-index tensors with fixed a are calculated in each loop.

$\langle ab|ef \rangle$ with fixed a is calculated as

$$V_{bf,e}^{[a]} = \sum_Q B_{[a]e}^Q B_{bf}^Q \quad (46)$$

$$(+)V_{b,e \geq f}^{[a]} = \frac{1}{2}(V_{bf,e}^{[a]} + V_{be,f}^{[a]}) \quad (47)$$

$$(-)V_{b,e \geq f}^{[a]} = \frac{1}{2}(V_{bf,e}^{[a]} - V_{be,f}^{[a]}) \quad (48)$$

For the contraction with the \hat{T}_2 amplitude, the symmetric/antisymmetric tensors are obtained as

$$S_{i \geq j,b}^{[a]} = \sum_{e \geq f} (+)T a u_{i \geq j}^{e \geq f} (+)V_{b,e \geq f}^{[a]} \quad (49)$$

$$A_{i \geq j,b}^{[a]} = \sum_{e \geq f} (-)T a u_{i \geq j}^{e \geq f} (-)V_{b,e \geq f}^{[a]} \quad (50)$$

After looping over a when limiting the summation to $a \geq b$, the contribution to the residual is calculated as

$$S_{i \geq j}^{a \geq b} + \epsilon_{ij} \epsilon_{ab} A_{i \geq j}^{a \geq b} \rightarrow R_{ij}^{ab} \quad (51)$$

4.6 \hat{T}_2 residual

With $W_{mnij}T_2$, $W_{mbej}T_2$, $W_{ijam}T_2$, and $W_{abef}T_2$ as parts of the \hat{T}_2 residual, we can write the whole residual as

$$R_{ij}^{ab} = P_{ij}^{ab} X_{ij}^{ab} + \langle ij|ab \rangle + W_{mnij}T_2 + W_{mbej}T_2 + W_{ijam}T_2 + W_{abef}T_2, \quad (52)$$

where

$$X_{ij}^{ab} = \sum_e t_{ij}^{ae} F_{be} - \sum_m t_{mj}^{ab} F_{mi} + \sum_Q t_{ia}^{'Q} B_{jb}^Q - \sum_Q t_{ai}^Q t_{jb}^Q \quad (53)$$

and

$$\langle ij|ab \rangle = \sum_Q B_{ia}^Q B_{jb}^Q. \quad (54)$$

Update the \hat{T}_2 amplitude,

$$t_{ij}^{ab} = t_{ij}^{ab} + R_{ij}^{ab}/D_{ij}^{ab}. \quad (55)$$

The denominator is defined as

$$D_{ij}^{ab} = \epsilon_a + \epsilon_b - \epsilon_i - \epsilon_j. \quad (56)$$

Note that the equations above can also match with Equation (10) to (16) in the reference as

$$\begin{aligned} R_{ij}^{ab} &= P_{ij}^{ab} X_{ij}^{ab} \\ &+ \langle ij|ab \rangle \Rightarrow \text{first term from non-}t_1\text{-transformed } B_{ia}^Q \\ &+ W_{mnij}T_2 \Rightarrow B_{ij}^{ab} \\ &+ W_{mbej}T_2 \Rightarrow C_{ij}^{ab} + D_{ij}^{ab} \\ &+ W_{ijam}T_2 \Rightarrow G_{ij}^{ab} \text{ except for the first term} \\ &+ W_{abef}T_2 \Rightarrow A_{ij}^{ab} + E_{ij}^{ab} \text{ except for the first term} \end{aligned} \quad (57)$$

and

$$\begin{aligned}
X_{ij}^{ab} &= \sum_e t_{ij}^{ae} F_{be} && \Rightarrow \text{first term in } E_{ij}^{ab} \\
&- \sum_m t_{mj}^{ab} F_{mi} && \Rightarrow \text{first term in } G_{ij}^{ab} \\
&+ \sum_Q t_{ia}^{Q} B_{jb}^Q - \sum_Q t_{ai}^Q t_{jb}^Q && \Rightarrow \text{first term from } t_1\text{-transformed } B_{ia}^Q \text{ that involves } t_1.
\end{aligned} \tag{58}$$

5 (T) correction

$$E_{(T)} = \frac{1}{3} \sum_{ijk} \sum_{abc} [(4W_{ijk}^{abc} + W_{ijk}^{bca}) + W_{ijk}^{cba}](V_{ijk}^{abc} - V_{ijk}^{cba})/D_{ijk}^{abc}, \tag{59}$$

where

$$W_{ijk}^{abc} = P_{ijk}^{abc} (\sum_e \langle ib|ae \rangle t_{jk}^{ec} - \sum_m \langle jm|kc \rangle t_{im}^{ab}), \tag{60}$$

$$V_{ijk}^{abc} = W_{ijk}^{abc} + t_i^a \langle jk|bc \rangle + t_j^b \langle ik|ac \rangle + t_k^c \langle ij|ab \rangle + f_{ia} t_{jk}^{bc} + f_{jb} t_{ik}^{ac} + f_{kc} t_{ij}^{ab}, \tag{61}$$

and

$$D_{ijk}^{abc} = \epsilon_a + \epsilon_b + \epsilon_c - \epsilon_i - \epsilon_j - \epsilon_k. \tag{62}$$

P_{ijk}^{abc} is the permutation operator defined as $P_{ijk}^{abc} X_{ijk}^{abc} = X_{ijk}^{abc} + X_{ikj}^{acb} + X_{jik}^{bac} + X_{jki}^{bca} + X_{kij}^{cab} + X_{kji}^{cba}$.

A few points in the implementation are worth mentioning:

- W and V intermediates are calculated for a fixed set of i, j, k and only $i \geq j \geq k$ for an efficient algorithm.
- four-index integrals that contain one or two virtual indices are calculated on-the-fly and stored in core.
- four-index integrals that contain three virtual indices are read in as N_V^3 tensors for a fixed i if they are stored out of core.
- $E_{(T)}$ is calculated for only $i \geq j \geq k$ and $a \geq b \geq c$.

Define

$$X_{ijk}^{abc} = P_{ijk}^{abc} (W_{abc}^{[ijk]} V_{abc}^{[ijk]}) \tag{63}$$

$$Y_{ijk}^{abc} = \tilde{V}_{abc}^{[ijk]} + \tilde{V}_{bca}^{[ijk]} + \tilde{V}_{cab}^{[ijk]} \tag{64}$$

$$Z_{ijk}^{abc} = \tilde{V}_{bac}^{[ijk]} + \tilde{V}_{cba}^{[ijk]} + \tilde{V}_{acb}^{[ijk]} \tag{65}$$

$$W^{(Y)} = W_{abc}^{[ijk]} + W_{bca}^{[ijk]} + W_{cab}^{[ijk]} \tag{66}$$

$$W^{(Z)} = W_{bac}^{[ijk]} + W_{cba}^{[ijk]} + W_{acb}^{[ijk]} \tag{67}$$

$$E_{(T)} = \sum_{i \geq j \geq k} \sum_{a \geq b \geq c} \frac{2 - (\delta_{ij} + \delta_{jk} + \delta_{ik})}{D_{ijk}^{abc}} [(Y - 2Z)W^{(Y)} + (Z - 2Y)W^{(Z)} + 3X] \tag{68}$$